'Verifier::visitInstruction' was done.
But we did not use 'ssreflect'. To connect the bool world and 
the logical world, for a particular relation, we must define both 
a boolean-version of this relation, and the Prop-version of this 
relation, and then use 'reflect' to connect them. Given a proposition, 
if the proposition is decidable, is there a way to generate its 
computational counterpart automatically? Coq doesn't allow us to 
destruct 'decidable' to return boolean, because boolean is in Set, 
while 'decidable'  is in Prop. I guess, this is how 'reflect' solved 
this problem? So I defined the two parts manually for each relation.

Ssreflect proved a lot of 'reflect' between logical connectives and 
the corresponding computational operations. say orP, with apply/orP 
and move/orP, we can switch between logical and computational. These 
apply/orP and move/orP tactics seem to be implemented by the extension 
of Coq core, not to be done with the existing Coq tactics.



git-svn-id: https://webdav.seas.upenn.edu/svn/sol/vol@2343 eef5ea85-cc2e-0410-bd84-0fae1f012da8

src/ssa/reflect.v
@@ -1,2 +1,59 @@
+Require Import ssa_lib.
+Require Import Decidable.
+
+Section Decidable.
+
+Lemma dec_blockDominates : forall (d:dt) (b1 b2: block),
+  decidable (blockDominates d b1 b2).
+Proof.
+  intros d b1 b2.
+  unfold decidable. unfold blockDominates.
+  destruct b1 as [l1 insns1].
+  destruct b2 as [l2 insns2].
+  remember (lset_mem l2 (d l1)) as c.
+  destruct c; auto.
+Qed.
+
+End Decidable.
+
+Inductive reflect (P:Prop) : bool -> Set :=
+| ReflectT : P -> reflect P true
+| ReflectF : ~P -> reflect P false
+.
+
+Section Reflect.
+
+Lemma reflect_blockDominates : forall d b1 b2,
+  reflect (blockDominates d b1 b2) (blockDominatesB d b1 b2).
+Proof.
+  intros d b1 b2.
+  unfold blockDominates. unfold blockDominatesB.
+  destruct b1 as [l1 insns1].
+  destruct b2 as [l2 insns2].
+  remember (lset_mem l2 (d l1)) as c.
+  destruct c; auto.
+    apply ReflectT; auto.
+    apply ReflectF; auto.
+Qed.
+
+Require Import Monad.
+
+Definition ifP d b1 b2 (X:Type) (t f : monad X) :=
+match (reflect_blockDominates d b1 b2) with
+| ReflectT _ => t
+| ReflectF _ => f
+end.
+
+End Reflect.
 
 
+
+
+
+
+(*
+*** Local Variables: ***
+*** coq-prog-name: "coqtop" ***
+*** coq-prog-args: ("-emacs-U" "-I" "./monads" "-I" "./ott") ***
+*** End: ***
+ *)
